Update a script to modern style, and speed up its slowest proof

examples/fun-op-sem/small-step/for_osmallScript.sml
@@ -10,14 +10,17 @@ val _ = new_theory "for_osmall";
 val ect = BasicProvers.EVERY_CASE_TAC;
 val fct = BasicProvers.FULL_CASE_TAC;
 
-val some_no_choice = Q.prove (
-`!f. (some x. f x) = NONE ⇔ ¬?x. f x`,
- rw [some_def]);
+Triviality some_no_choice:
+  !f. (some x. f x) = NONE ⇔ ¬?x. f x
+Proof rw [some_def]
+QED
 
-val some_SAT = Q.prove(
-`!P y. (some x. P x) = SOME y ⇒ P y`,
-rw[some_def,SELECT_THM]>>
-metis_tac[SELECT_AX])
+Triviality some_SAT:
+  !P y. (some x. P x) = SOME y ⇒ P y
+Proof
+  rw[some_def,SELECT_THM]>>
+  metis_tac[SELECT_AX]
+QED
 
 (* A small step semantics for the non-deterministic FOR language with I/O *)
 
@@ -138,10 +141,11 @@ Inductive step_e:
             (s with io_trace := s.io_trace ++ [INL (Otag i)], Num i))
 End
 
-val is_val_t_def = Define `
-(is_val_t (Exp (e : small_e)) = is_val_e e) ∧
-(is_val_t Break = T) ∧
-(is_val_t _ = F)`;
+Definition is_val_t_def:
+  (is_val_t (Exp (e : small_e)) = is_val_e e) ∧
+  (is_val_t Break = T) ∧
+  (is_val_t _ = F)
+End
 
 Inductive step_t:
   (!s t x.
@@ -278,7 +282,9 @@ Inductive res_rel_e:
     res_rel_e (Rfail, s) (s with clock:=0, e))
 End
 
-val conjs_def = Define` conjs A B ⇔ A ∧ B`
+Definition conjs_def:
+  conjs A B ⇔ A ∧ B
+End
 
 val etac = (fs[Once step_t_cases]>>fs[Once step_t_cases,Once step_e_cases,conjs_def])
 
@@ -333,8 +339,8 @@ Proof
   >- etac
   >-
     (fs[Once step_t_cases]>>rfs[conjs_def]>>
-    Cases_on`t`>>fs[is_val_t_def]>>
-    Cases_on`s'`>>fs[is_val_e_def]>>
+    Cases_on‘t’>>fs[is_val_t_def]>>
+    Cases_on‘s'’>>fs[is_val_e_def]>>
     fs[Once step_t_cases]>>
     fs[Once step_e_cases])
   >-
@@ -343,7 +349,7 @@ Proof
     >-
       etac
     >-
-      (Cases_on`t1`>>fs[is_val_t_def]>>Cases_on`s`>>fs[is_val_e_def]>>
+      (Cases_on‘t1’>>fs[is_val_t_def]>>Cases_on‘s’>>fs[is_val_e_def]>>
       fs[Once step_t_cases,Once step_e_cases])
     >>
       fs[FORALL_PROD]>>metis_tac[])
@@ -375,8 +381,8 @@ Theorem check_trace_seq:
                 (MAP (λst,t. (st,Seq t p)) tr)
 Proof
  Induct>>rw[]>>
- Cases_on`tr`>>fs[check_trace_def]>>
- Cases_on`h`>>Cases_on`h'`>>
+ Cases_on‘tr’>>fs[check_trace_def]>>
+ Cases_on‘h’>>Cases_on‘h'’>>
  match_mp_tac some_to_SOME_step_t>>
  fs[some_def]>>
  simp[Once step_t_cases]>>
@@ -389,8 +395,8 @@ Theorem check_trace_assign:
     check_trace (λst. some st'. ?l. step_e st l st')
                 (MAP (λ(st,e). (st,Assign s e)) tr)
 Proof
- Induct>>rw[]>>Cases_on`tr`>>fs[check_trace_def]>>
- Cases_on`h`>>Cases_on`h'`>>
+ Induct>>rw[]>>Cases_on‘tr’>>fs[check_trace_def]>>
+ Cases_on‘h’>>Cases_on‘h'’>>
  match_mp_tac some_to_SOME_step_e>>
  fs[some_def]>>
  simp[Once step_e_cases]>>
@@ -403,8 +409,8 @@ Theorem check_trace_putchar:
     check_trace (λst. some st'. ?l. step_e st l st')
                 (MAP (λ(st,e). (st,Putchar e)) tr)
 Proof
- Induct>>rw[]>>Cases_on`tr`>>fs[check_trace_def]>>
- Cases_on`h`>>Cases_on`h'`>>
+ Induct>>rw[]>>Cases_on‘tr’>>fs[check_trace_def]>>
+ Cases_on‘h’>>Cases_on‘h'’>>
  match_mp_tac some_to_SOME_step_e>>
  fs[some_def]>>
  simp[Once step_e_cases]>>
@@ -417,8 +423,8 @@ Theorem check_trace_addl1:
     check_trace (λst. some st'. ?l. step_e st l st')
                 (MAP (λst,e. (st,AddL e e')) tr)
 Proof
- Induct>>rw[]>>Cases_on`tr`>>fs[check_trace_def]>>
- Cases_on`h`>>Cases_on`h'`>>
+ Induct>>rw[]>>Cases_on‘tr’>>fs[check_trace_def]>>
+ Cases_on‘h’>>Cases_on‘h'’>>
  match_mp_tac some_to_SOME_step_e>>
  fs[some_def]>>
  simp[Once step_e_cases]>>
@@ -431,8 +437,8 @@ Theorem check_trace_addl2:
     check_trace (λst. some st'. ?l. step_e st l st')
                 (MAP (λ(st,e'). (st,AddL (Num i) e')) tr)
 Proof
- Induct>>rw[]>>Cases_on`tr`>>fs[check_trace_def]>>
- Cases_on`h`>>Cases_on`h'`>>
+ Induct>>rw[]>>Cases_on‘tr’>>fs[check_trace_def]>>
+ Cases_on‘h’>>Cases_on‘h'’>>
  match_mp_tac some_to_SOME_step_e>>
  fs[some_def]>>
  simp[Once step_e_cases]>>
@@ -445,8 +451,8 @@ Theorem check_trace_addr1:
     check_trace (λst. some st'. ?l. step_e st l st')
                 (MAP (λ(st,e'). (st,AddR e e')) tr)
 Proof
- Induct>>rw[]>>Cases_on`tr`>>fs[check_trace_def]>>
- Cases_on`h`>>Cases_on`h'`>>
+ Induct>>rw[]>>Cases_on‘tr’>>fs[check_trace_def]>>
+ Cases_on‘h’>>Cases_on‘h'’>>
  match_mp_tac some_to_SOME_step_e>>
  fs[some_def]>>
  simp[Once step_e_cases]>>
@@ -459,8 +465,8 @@ Theorem check_trace_addr2:
     check_trace (λst. some st'. ?l. step_e st l st')
                 (MAP (λst,e'. (st,AddR e' (Num i))) tr)
 Proof
- Induct>>rw[]>>Cases_on`tr`>>fs[check_trace_def]>>
- Cases_on`h`>>Cases_on`h'`>>
+ Induct>>rw[]>>Cases_on‘tr’>>fs[check_trace_def]>>
+ Cases_on‘h’>>Cases_on‘h'’>>
  match_mp_tac some_to_SOME_step_e>>
  fs[some_def]>>
  simp[Once step_e_cases]>>
@@ -473,8 +479,8 @@ Theorem check_trace_exp:
     check_trace (λst. some st'. ?l. step_t st l st')
                 (MAP (λst,e'. (st,Exp e')) tr)
 Proof
- Induct>>rw[check_trace_def]>>Cases_on`tr`>>fs[check_trace_def]>>
- Cases_on`h`>>Cases_on`h'`>>
+ Induct>>rw[check_trace_def]>>Cases_on‘tr’>>fs[check_trace_def]>>
+ Cases_on‘h’>>Cases_on‘h'’>>
  match_mp_tac some_to_SOME_step_t>>
  fs[some_def]>>
  simp[Once step_t_cases]>>
@@ -487,8 +493,8 @@ Theorem check_trace_if1:
     check_trace (λst. some st'. ?l. step_t st l st')
                 (MAP (λst,e'. (st,If e' a b)) tr)
 Proof
- Induct>>rw[check_trace_def]>>Cases_on`tr`>>fs[check_trace_def]>>
- Cases_on`h`>>Cases_on`h'`>>
+ Induct>>rw[check_trace_def]>>Cases_on‘tr’>>fs[check_trace_def]>>
+ Cases_on‘h’>>Cases_on‘h'’>>
  match_mp_tac some_to_SOME_step_t>>
  fs[some_def]>>
  simp[Once step_t_cases]>>
@@ -501,8 +507,8 @@ Theorem check_trace_for1:
     check_trace (λst. some st'. ?l. step_t st l st')
                 (MAP (λst,e'. (st, Handle (If e' a b))) tr)
 Proof
-  Induct>>rw[check_trace_def]>>Cases_on`tr`>>fs[check_trace_def]>>
-  Cases_on`h`>>Cases_on`h'`>>
+  Induct>>rw[check_trace_def]>>Cases_on‘tr’>>fs[check_trace_def]>>
+  Cases_on‘h’>>Cases_on‘h'’>>
           match_mp_tac some_to_SOME_step_t>>
   fs[some_def]>>
   simp[Once step_t_cases]>>
@@ -516,8 +522,8 @@ Theorem check_trace_for2:
     check_trace (λst. some st'. ?l. step_t st l st')
                 (MAP (λst,t'. (st, Handle (Seq t' a))) tr)
 Proof
- Induct>>rw[check_trace_def]>>Cases_on`tr`>>fs[check_trace_def]>>
- Cases_on`h`>>Cases_on`h'`>>
+ Induct>>rw[check_trace_def]>>Cases_on‘tr’>>fs[check_trace_def]>>
+ Cases_on‘h’>>Cases_on‘h'’>>
  match_mp_tac some_to_SOME_step_t>>
  fs[some_def]>>
  simp[Once step_t_cases]>>
@@ -531,8 +537,8 @@ Theorem check_trace_for3:
     check_trace (λst. some st'. ?l. step_t st l st')
                 (MAP (λst,e'. (st, Handle (Seq (Exp e') a))) tr)
 Proof
- Induct>>rw[check_trace_def]>>Cases_on`tr`>>fs[check_trace_def]>>
- Cases_on`h`>>Cases_on`h'`>>
+ Induct>>rw[check_trace_def]>>Cases_on‘tr’>>fs[check_trace_def]>>
+ Cases_on‘h’>>Cases_on‘h'’>>
  match_mp_tac some_to_SOME_step_t>>
  fs[some_def]>>
  ntac 3 (simp[Once step_t_cases])>>
@@ -545,12 +551,12 @@ Theorem check_trace_handle:
     check_trace (λst. some st'. ?l. step_t st l st')
                 (MAP (λst,t'. (st, Handle t')) tr)
 Proof
- Induct>>rw[check_trace_def]>>Cases_on`tr`>>fs[check_trace_def]>>
- Cases_on`h`>>Cases_on`h'`>>
+ Induct>>rw[check_trace_def]>>Cases_on‘tr’>>fs[check_trace_def]>>
+ Cases_on‘h’>>Cases_on‘h'’>>
  match_mp_tac some_to_SOME_step_t>>
  fs[some_def]>>
  simp[Once step_t_cases]>>
- Cases_on`st'`>>metis_tac[step_t_determ]
+ Cases_on‘st'’>>metis_tac[step_t_determ]
 QED
 
 (* Non-existence of contextual transitions in small-step *)
@@ -634,7 +640,7 @@ Theorem no_step_t_seq:
 Proof
  Induct>>rw[is_val_t_def]>>
  simp[Once step_t_cases]>>
- Cases_on`s'`>>fs[is_val_e_def]
+ Cases_on‘s'’>>fs[is_val_e_def]
 QED
 
 Theorem no_step_t_if1:
@@ -664,55 +670,65 @@ Proof Cases >> rw[]
 QED
 
 Theorem HD_APPEND[local]: ls ≠ [] ⇒ HD (ls ++ ls') = HD ls
-Proof Cases_on`ls`>>fs[]
+Proof Cases_on‘ls’>>fs[]
 QED
 
 Theorem LAST_APPEND[local]: ls' ≠ [] ⇒ LAST (ls ++ ls') = LAST ls'
-Proof Cases_on`ls'`>>fs[]
+Proof Cases_on‘ls'’>>fs[]
 QED
 
-val sem_e_not_timeout = Q.prove (
-`!st e r. sem_e st e ≠ (Rtimeout, r)`,
- Induct_on `e` >>
- rw [sem_e_def, LET_THM, permute_pair_def, oracle_get_def, unpermute_pair_def, getchar_def] >>
- ect >>
- fs [] >>
- metis_tac []);
+Triviality sem_e_not_timeout:
+  !st e r. sem_e st e ≠ (Rtimeout, r)
+Proof
+  Induct_on ‘e’ >>
+  rw [sem_e_def, LET_THM, permute_pair_def, oracle_get_def, unpermute_pair_def,
+      getchar_def] >>
+  ect >>
+  fs [] >>
+  metis_tac []
+QED
 
-val sem_e_not_break = Q.prove(
-`!st e r. sem_e st e ≠ (Rbreak,r)`,
-  Induct_on`e`>>srw_tac[][sem_e_def]>>
+Triviality sem_e_not_break:
+  !st e r. sem_e st e ≠ (Rbreak,r)
+Proof
+  Induct_on‘e’>>srw_tac[][sem_e_def]>>
   ect>>
   fs[LET_THM,unpermute_pair_def,permute_pair_def,oracle_get_def] >>
-  qpat_x_assum `_ = (fst_e,snd_e)` mp_tac >> rw[] >>
-  rename1 `sem_e st' _ = (Rbreak, new_r)` >>
-  first_x_assum (qspecl_then [`st'`,`new_r`] assume_tac) >>
-  first_x_assum (qspecl_then [`st'`,`new_r`] assume_tac) >>
+  qpat_x_assum ‘_ = (fst_e,snd_e)’ mp_tac >> rw[] >>
+  rename1 ‘sem_e st' _ = (Rbreak, new_r)’ >>
+  first_x_assum (qspecl_then [‘st'’,‘new_r’] assume_tac) >>
+  first_x_assum (qspecl_then [‘st'’,‘new_r’] assume_tac) >>
   fs[]
- );
+QED
 
-val LAST_HD_eq = Q.prove(`
-∀ls ls'.
- ls ≠ [] ∧ ls' ≠ [] ∧
- LAST ls = HD ls' ⇒
- BUTLASTN 1 ls ++ ls' =
- ls ++ TL ls'`,
- Induct>>fs[LAST_DEF,BUTLASTN_1]>>rw[]>>
- Cases_on`ls'`>>fs[FRONT_DEF])
+Triviality LAST_HD_eq:
+  ∀ls ls'.
+    ls ≠ [] ∧ ls' ≠ [] ∧
+    LAST ls = HD ls' ⇒
+    BUTLASTN 1 ls ++ ls' =
+    ls ++ TL ls'
+Proof
+  Induct>>fs[LAST_DEF,BUTLASTN_1]>>rw[]>>
+  Cases_on‘ls'’>>fs[FRONT_DEF]
+QED
 
-val check_trace_append3 = Q.prove(`
- check_trace f ls ∧
- f h = SOME (HD ls) ⇒
- check_trace f (h :: ls)`,
- rw[]>>imp_res_tac check_trace_append2>>
- pop_assum(qspec_then`[h]`assume_tac)>>fs[]>>
- rfs[check_trace_def])
+Triviality check_trace_append3:
+  check_trace f ls ∧
+  f h = SOME (HD ls) ⇒
+  check_trace f (h :: ls)
+Proof
+  rw[]>>imp_res_tac check_trace_append2>>
+  pop_assum(qspec_then‘[h]’assume_tac)>>fs[]>>
+  rfs[check_trace_def]
+QED
 
-val check_trace_tl = Q.prove(`
- check_trace f ls ∧ ls ≠ [] ⇒
- check_trace f (TL ls)`,
- Cases_on`ls`>>fs[check_trace_def]>>
- Cases_on`t`>>fs[check_trace_def])
+Triviality check_trace_tl:
+  check_trace f ls ∧ ls ≠ [] ⇒
+  check_trace f (TL ls)
+Proof
+  Cases_on‘ls’>>fs[check_trace_def]>>
+  Cases_on‘t’>>fs[check_trace_def]
+QED
 
 (* Start connecting functional big step to small step traces *)
 local val rw = srw_tac[] val fs = fsrw_tac[] in
@@ -724,55 +740,55 @@ Theorem sem_e_big_small_lem[local]:
             HD tr = (s with clock:=0, e_to_small_e e) ∧
             res_rel_e r (LAST tr)
 Proof
- Induct_on`e`>>rw[]>>fs[sem_e_def,e_to_small_e_def]
+ Induct_on‘e’>>rw[]>>fs[sem_e_def,e_to_small_e_def]
   >- (
     fct>>fs[res_rel_e_cases]
     >- (
-      qexists_tac`[(s' with clock:=0,Var s)]`>>fs[check_trace_def,is_val_e_def]>>
+      qexists_tac‘[(s' with clock:=0,Var s)]’>>fs[check_trace_def,is_val_e_def]>>
       simp[Once step_e_cases]
       )
     >- (
-      qexists_tac`[(s' with clock:=0,Var s);(s' with clock:=0,Num x)]`>>
+      qexists_tac‘[(s' with clock:=0,Var s);(s' with clock:=0,Num x)]’>>
       fs[check_trace_def,some_def]>>
       ntac 2 (simp[Once step_e_cases])
       )
     )
   >- (
     fs[res_rel_e_cases]>>
-    qexists_tac`[s with clock:=0,Num i]`>>fs[check_trace_def]
+    qexists_tac‘[s with clock:=0,Num i]’>>fs[check_trace_def]
     )
   >- (
     fs[LET_THM,permute_pair_def,oracle_get_def]>>IF_CASES_TAC>>fs[]
     >- (
-      qpat_abbrev_tac`st = s with <|io_trace:=B;non_det_o:=C|>`>>
-      first_x_assum(qspec_then`st`assume_tac)>>
-      Cases_on`sem_e st e'`>>Cases_on`q`>>
+      qpat_abbrev_tac‘st = s with <|io_trace:=B;non_det_o:=C|>’>>
+      first_x_assum(qspec_then‘st’assume_tac)>>
+      Cases_on‘sem_e st e'’>>Cases_on‘q’>>
       fs[sem_e_not_break,sem_e_not_timeout,unpermute_pair_def]
       >- (
-        fct>>Cases_on`q`>>
+        fct>>Cases_on‘q’>>
         fs[sem_e_not_break,sem_e_not_timeout]>>
-        last_x_assum(qspec_then`r` assume_tac)>>rfs[]>>
-        qpat_abbrev_tac`h =(A,B)`>>
-        qabbrev_tac`ls1 = (MAP (λst,e'. (st,AddR (e_to_small_e e) e')) tr)`>>
-        qabbrev_tac`ls2 = (MAP (λst,e'. (st,AddR e' (Num i))) tr')`>>
-        qabbrev_tac`ls = BUTLASTN 1 ls1 ++ ls2`>>
+        last_x_assum(qspec_then‘r’ assume_tac)>>rfs[]>>
+        qpat_abbrev_tac‘h =(A,B)’>>
+        qabbrev_tac‘ls1 = (MAP (λst,e'. (st,AddR (e_to_small_e e) e')) tr)’>>
+        qabbrev_tac‘ls2 = (MAP (λst,e'. (st,AddR e' (Num i))) tr')’>>
+        qabbrev_tac‘ls = BUTLASTN 1 ls1 ++ ls2’>>
         fs[res_rel_e_cases]>>
-        `LAST ls1 = HD ls2` by (unabbrev_all_tac>>fs[LAST_MAP,HD_MAP])>>
-        `ls = ls1 ++ (TL ls2)` by (unabbrev_all_tac>> fs[LAST_HD_eq])>>
-        `check_trace (λst. some st'. ∃l. step_e st l st') ls2` by
-          fs[Abbr`ls2`,check_trace_addr2]>>
-        `check_trace (λst. some st'. ∃l. step_e st l st') ls`
-          by (fs[Abbr`ls`]>>Cases_on`ls2`>>fs[]>>Cases_on`t`>>fs[]
-              >- fs[check_trace_addr1,Abbr`ls1`] >>
+        ‘LAST ls1 = HD ls2’ by (unabbrev_all_tac>>fs[LAST_MAP,HD_MAP])>>
+        ‘ls = ls1 ++ (TL ls2)’ by (unabbrev_all_tac>> fs[LAST_HD_eq])>>
+        ‘check_trace (λst. some st'. ∃l. step_e st l st') ls2’ by
+          fs[Abbr‘ls2’,check_trace_addr2]>>
+        ‘check_trace (λst. some st'. ∃l. step_e st l st') ls’
+          by (fs[Abbr‘ls’]>>Cases_on‘ls2’>>fs[]>>Cases_on‘t’>>fs[]
+              >- fs[check_trace_addr1,Abbr‘ls1’] >>
               match_mp_tac check_trace_append2>>rw[]
-              >- fs[check_trace_addr1,Abbr`ls1`]
+              >- fs[check_trace_addr1,Abbr‘ls1’]
               >- (fs[markerTheory.Abbrev_def]>>
-                  `h''::t' = TL (LAST ls1::h''::t')` by fs[]>>
+                  ‘h''::t' = TL (LAST ls1::h''::t')’ by fs[]>>
                   pop_assum SUBST_ALL_TAC>>
                   match_mp_tac check_trace_tl>>fs[check_trace_addr2]) >>
               fs[check_trace_def])
         >- (
-          qexists_tac`[h] ++ ls ++ [(r' with clock:=0,Num(i'+i))]`>>
+          qexists_tac‘[h] ++ ls ++ [(r' with clock:=0,Num(i'+i))]’>>
           rw[]>>
           match_mp_tac check_trace_append3>>fs[check_trace_def]>>rw[]
           >- (
@@ -784,15 +800,15 @@ Proof
             simp[Once step_e_cases]
             ) >>
           match_mp_tac some_to_SOME_step_e>>
-          fs[HD_APPEND,Abbr`ls1`,HD_MAP,Abbr`h`,Abbr`st`]>>
+          fs[HD_APPEND,Abbr‘ls1’,HD_MAP,Abbr‘h’,Abbr‘st’]>>
           simp[Once step_e_cases,oracle_get_def]
           ) >>
-        qexists_tac`[h]++ls` >>rw[]
+        qexists_tac‘[h]++ls’ >>rw[]
         >- (
           match_mp_tac check_trace_append3>>
-          fs[HD_APPEND,Abbr`ls1`,HD_MAP]>>
+          fs[HD_APPEND,Abbr‘ls1’,HD_MAP]>>
           match_mp_tac some_to_SOME_step_e>>
-          fs[Abbr`h`,Abbr`st`]>>
+          fs[Abbr‘h’,Abbr‘st’]>>
           simp[Once step_e_cases,oracle_get_def]
           ) >>
         qpat_x_assum ‘BUTLASTN 1 _ ++ _ = _’ (REWRITE_TAC o single o SYM) >>
@@ -800,8 +816,8 @@ Proof
            is_val_e_def,no_step_e_addr2]
         )
       >- (
-        qpat_abbrev_tac`h =(A,B)`>>
-        qexists_tac`[h]++(MAP (λst,e'. (st,AddR (e_to_small_e e) e')) tr)`>>
+        qpat_abbrev_tac‘h =(A,B)’>>
+        qexists_tac‘[h]++(MAP (λst,e'. (st,AddR (e_to_small_e e) e')) tr)’>>
         fs[HD_MAP,res_rel_e_cases,LAST_MAP,is_val_e_def,
            LAST_APPEND,no_step_e_addr1]>>
         match_mp_tac check_trace_append3>>fs[check_trace_addr1,HD_MAP]>>
@@ -812,38 +828,38 @@ Proof
       )
     >- (
       (*symmetric*)
-      qpat_abbrev_tac`st = s with <|io_trace:=B;non_det_o:=C|>`>>
-      last_x_assum(qspec_then`st`assume_tac)>>
-      Cases_on`sem_e st e`>>Cases_on`q`>>
+      qpat_abbrev_tac‘st = s with <|io_trace:=B;non_det_o:=C|>’>>
+      last_x_assum(qspec_then‘st’assume_tac)>>
+      Cases_on‘sem_e st e’>>Cases_on‘q’>>
       fs[sem_e_not_break,sem_e_not_timeout,unpermute_pair_def]
       >- (
-        fct>>Cases_on`q`>>
+        fct>>Cases_on‘q’>>
         fs[sem_e_not_break,sem_e_not_timeout]>>
-        last_x_assum(qspec_then`r` assume_tac)>>rfs[]>>
-        qpat_abbrev_tac`h =(A,B)`>>
-        qabbrev_tac`ls1 = (MAP (λst,e. (st,AddL e (e_to_small_e e'))) tr)`>>
-        qabbrev_tac`ls2 = (MAP (λst,e'. (st,AddL (Num i) e')) tr')`>>
-        qabbrev_tac`ls = BUTLASTN 1 ls1 ++ ls2`>>
+        last_x_assum(qspec_then‘r’ assume_tac)>>rfs[]>>
+        qpat_abbrev_tac‘h =(A,B)’>>
+        qabbrev_tac‘ls1 = (MAP (λst,e. (st,AddL e (e_to_small_e e'))) tr)’>>
+        qabbrev_tac‘ls2 = (MAP (λst,e'. (st,AddL (Num i) e')) tr')’>>
+        qabbrev_tac‘ls = BUTLASTN 1 ls1 ++ ls2’>>
         fs[res_rel_e_cases]>>
-        `LAST ls1 = HD ls2` by (unabbrev_all_tac>>fs[LAST_MAP,HD_MAP])>>
-        `ls = ls1 ++ (TL ls2)` by (unabbrev_all_tac>> fs[LAST_HD_eq])>>
-        `check_trace (λst. some st'. ∃l. step_e st l st') ls2` by
-        fs[Abbr`ls2`,check_trace_addl2]>>
-        `check_trace (λst. some st'. ∃l. step_e st l st') ls` by (
-          fs[Abbr`ls`]>>Cases_on`ls2`>>fs[]>>Cases_on`t`>>fs[]
-          >- fs[check_trace_addl1,Abbr`ls1`] >>
+        ‘LAST ls1 = HD ls2’ by (unabbrev_all_tac>>fs[LAST_MAP,HD_MAP])>>
+        ‘ls = ls1 ++ (TL ls2)’ by (unabbrev_all_tac>> fs[LAST_HD_eq])>>
+        ‘check_trace (λst. some st'. ∃l. step_e st l st') ls2’ by
+        fs[Abbr‘ls2’,check_trace_addl2]>>
+        ‘check_trace (λst. some st'. ∃l. step_e st l st') ls’ by (
+          fs[Abbr‘ls’]>>Cases_on‘ls2’>>fs[]>>Cases_on‘t’>>fs[]
+          >- fs[check_trace_addl1,Abbr‘ls1’] >>
           match_mp_tac check_trace_append2>>rw[]
-          >- fs[check_trace_addl1,Abbr`ls1`]
+          >- fs[check_trace_addl1,Abbr‘ls1’]
           >- (
             fs[markerTheory.Abbrev_def]>>
-            `h''::t' = TL (LAST ls1::h''::t')` by fs[]>>
+            ‘h''::t' = TL (LAST ls1::h''::t')’ by fs[]>>
             pop_assum SUBST_ALL_TAC>>
             match_mp_tac check_trace_tl>>fs[check_trace_addr2]
             ) >>
           fs[check_trace_def]
           )
         >- (
-          qexists_tac`[h] ++ ls ++ [(r' with clock:=0,Num(i+i'))]`>>
+          qexists_tac‘[h] ++ ls ++ [(r' with clock:=0,Num(i+i'))]’>>
           rw[]>>
           match_mp_tac check_trace_append3>>fs[check_trace_def]>>rw[]
           >- (
@@ -855,16 +871,16 @@ Proof
             simp[Once step_e_cases]
             ) >>
           match_mp_tac some_to_SOME_step_e>>
-          fs[HD_APPEND,Abbr`ls1`,HD_MAP,Abbr`h`,Abbr`st`]>>
+          fs[HD_APPEND,Abbr‘ls1’,HD_MAP,Abbr‘h’,Abbr‘st’]>>
           simp[Once step_e_cases,oracle_get_def]
           )
         >- (
-          qexists_tac`[h]++ls` >>rw[]
+          qexists_tac‘[h]++ls’ >>rw[]
           >- (
             match_mp_tac check_trace_append3>>
-            fs[HD_APPEND,Abbr`ls1`,HD_MAP]>>
+            fs[HD_APPEND,Abbr‘ls1’,HD_MAP]>>
             match_mp_tac some_to_SOME_step_e>>
-            fs[Abbr`h`,Abbr`st`]>>
+            fs[Abbr‘h’,Abbr‘st’]>>
             simp[Once step_e_cases,oracle_get_def]
             ) >>
           qpat_x_assum ‘BUTLASTN _ _ ++ _ = _’ (REWRITE_TAC o single o SYM) >>
@@ -873,8 +889,8 @@ Proof
           )
         )
       >- (
-        qpat_abbrev_tac`h =(A,B)`>>
-        qexists_tac`[h]++(MAP (λst,e. (st,AddL e (e_to_small_e e'))) tr)`>>
+        qpat_abbrev_tac‘h =(A,B)’>>
+        qexists_tac‘[h]++(MAP (λst,e. (st,AddL e (e_to_small_e e'))) tr)’>>
         fs[HD_MAP,res_rel_e_cases,LAST_MAP,is_val_e_def,LAST_APPEND,
            no_step_e_addl1]>>
         match_mp_tac check_trace_append3>>fs[check_trace_addl1,HD_MAP]>>
@@ -886,104 +902,111 @@ Proof
     )
   >- (
     EVERY_CASE_TAC>>fs[res_rel_e_cases,sem_e_not_break,sem_e_not_timeout]>>
-    first_x_assum(qspec_then`s'` assume_tac)>>rfs[]
+    first_x_assum(qspec_then‘s'’ assume_tac)>>rfs[]
     >- (
-      qexists_tac`(MAP (λst,e. (st,Assign s e)) tr)++
-        [r with <|store :=r.store |+ (s,i); clock:=0|>,Num i]`>>
+      qexists_tac‘(MAP (λst,e. (st,Assign s e)) tr)++
+        [r with <|store :=r.store |+ (s,i); clock:=0|>,Num i]’>>
       fs[HD_MAP,HD_APPEND]>>
       ho_match_mp_tac check_trace_append2>>
       fs[check_trace_def,LAST_MAP,check_trace_assign]>>
       ntac 2 (simp[Once step_e_cases])
       ) >>
       (
-        qexists_tac`(MAP (λst,e. (st,Assign s e)) tr)`>>
+        qexists_tac‘(MAP (λst,e. (st,Assign s e)) tr)’>>
         fs[HD_MAP,LAST_MAP,is_val_e_def,no_step_e_assign,check_trace_assign]
       )
     )
   >- (
-    Cases_on`getchar s.input`>>fs[LET_THM,res_rel_e_cases]>>
-    qpat_abbrev_tac`t = (A,B)`>>
-    qpat_abbrev_tac`t' = (A,B)`>>
-    qexists_tac`[t;t']`>>unabbrev_all_tac>>fs[check_trace_def]>>
+    Cases_on‘getchar s.input’>>fs[LET_THM,res_rel_e_cases]>>
+    qpat_abbrev_tac‘t = (A,B)’>>
+    qpat_abbrev_tac‘t' = (A,B)’>>
+    qexists_tac‘[t;t']’>>unabbrev_all_tac>>fs[check_trace_def]>>
     match_mp_tac some_to_SOME_step_e>>
     simp[Once step_e_cases]
     )
   >- (
-    first_x_assum(qspec_then`s` assume_tac)>>fs[]>>
-    Cases_on`sem_e s e`>>Cases_on`q`>>fs[sem_e_not_break,sem_e_not_timeout]>>
-    qpat_abbrev_tac`t = (A,B)`>>
-    qpat_abbrev_tac`t' = (A,B)`
+    first_x_assum(qspec_then‘s’ assume_tac)>>fs[]>>
+    Cases_on‘sem_e s e’>>Cases_on‘q’>>fs[sem_e_not_break,sem_e_not_timeout]>>
+    qpat_abbrev_tac‘t = (A,B)’>>
+    qpat_abbrev_tac‘t' = (A,B)’
     >- (
-      qexists_tac`MAP (λst,e. (st,Putchar e)) tr ++
-        [(r with <|io_trace := r.io_trace ++ [INL(Otag i)];clock:=0|>,Num i)]`>>
-      fs[HD_MAP,HD_APPEND,Abbr`t'`,res_rel_e_cases]>>
+      qexists_tac‘MAP (λst,e. (st,Putchar e)) tr ++
+        [(r with <|io_trace := r.io_trace ++ [INL(Otag i)];clock:=0|>,Num i)]’>>
+      fs[HD_MAP,HD_APPEND,Abbr‘t'’,res_rel_e_cases]>>
       ho_match_mp_tac check_trace_append2>>
       fs[check_trace_def,LAST_MAP,check_trace_putchar]>>
       ntac 2 (simp[Once step_e_cases])
       ) >>
-    qexists_tac`MAP (λst,e. (st,Putchar e)) tr`>>unabbrev_all_tac>>
+    qexists_tac‘MAP (λst,e. (st,Putchar e)) tr’>>unabbrev_all_tac>>
     fs[HD_MAP,res_rel_e_cases,LAST_MAP,is_val_e_def,check_trace_putchar,
        no_step_e_putchar]
     )
 QED
 end
 
-val sem_t_for_no_break = Q.prove(
- `∀s s'. sem_t s (For e1 e2 t) ≠ (Rbreak,s')`,
- completeInduct_on`s.clock`>>fs[sem_t_def_with_stop]>>
- rw[]>>fct>>Cases_on`q`>>
+Triviality sem_t_for_no_break:
+  ∀s s'. sem_t s (For e1 e2 t) ≠ (Rbreak,s')
+Proof
+ completeInduct_on‘s.clock’>>fs[sem_t_def_with_stop]>>
+ rw[]>>fct>>Cases_on‘q’>>
  fs[sem_e_not_break,sem_e_not_timeout]>>
  IF_CASES_TAC>>fs[]>>
- fct>>Cases_on`q`>>fs[]>>
- fct>>Cases_on`q`>>fs[sem_e_not_break,sem_e_not_timeout]>>
+ fct>>Cases_on‘q’>>fs[]>>
+ fct>>Cases_on‘q’>>fs[sem_e_not_break,sem_e_not_timeout]>>
  imp_res_tac sem_e_clock>>imp_res_tac sem_t_clock>>fs[]>>
  IF_CASES_TAC>>fs[dec_clock_def]>>
  simp[STOP_def]>>
  simp[sem_t_def_with_stop]>>
  fs[PULL_FORALL]>>
- first_x_assum(qspec_then `r'' with clock := r''.clock-1` mp_tac)>>
+ first_x_assum(qspec_then ‘r'' with clock := r''.clock-1’ mp_tac)>>
  fs[]>>
- `r''.clock < 1 + r.clock ∧ 0 < r.clock` by
+ ‘r''.clock < 1 + r.clock ∧ 0 < r.clock’ by
    DECIDE_TAC>>
- fs[dec_clock_def])
+ fs[dec_clock_def]
+QED
 
-val step_e_clock = Q.prove(`
+Triviality step_e_clock:
   ∀se l1 se'.
-  step_e se l1 se' ⇒
-  ∀s e s' e'.
-  se = (s,e) ∧
-  se' = (s',e') ⇒
-  (∀c.
-  step_e (s with clock:=c,e) l1 (s' with clock:=c,e'))`,
+    step_e se l1 se' ⇒
+    ∀s e s' e'.
+      se = (s,e) ∧
+      se' = (s',e') ⇒
+      ∀c.
+         step_e (s with clock:=c,e) l1 (s' with clock:=c,e')
+Proof
   ho_match_mp_tac step_e_strongind>>rw[]>>
-  simp[Once step_e_cases])
+  simp[Once step_e_cases]
+QED
 
-val step_e_zero_clock = Q.prove(
- `(∀s e l. ¬step_e (r,e') l (s,e))⇒
- ∀s e l. ¬step_e (r with clock:=0,e') l (s,e)`,
- rw[]>>CCONTR_TAC>>fs[]>>imp_res_tac step_e_clock>>fs[]>>
- pop_assum(qspec_then`r.clock`assume_tac)>>fs[]>>
- `r with clock:= r.clock = r` by fs[state_component_equality]>>
- metis_tac[])
+Triviality step_e_zero_clock:
+  (∀s e l. ¬step_e (r,e') l (s,e)) ⇒
+  ∀s e l. ¬step_e (r with clock:=0,e') l (s,e)
+Proof
+  rw[]>>CCONTR_TAC>>fs[]>>imp_res_tac step_e_clock>>fs[]>>
+  pop_assum(qspec_then‘r.clock’assume_tac)>>fs[]>>
+  ‘r with clock:= r.clock = r’ by fs[state_component_equality]>>
+  metis_tac[]
+QED
 
-val big_small_lem = Q.prove (
-`!s t r.
-  sem_t s t = r
-  ⇒
-  ?tr.
-    tr ≠ [] ∧
-    s.clock - (SND r).clock ≤ LENGTH tr ∧
-    check_trace (\st. some st'. ?l. step_t st l st') tr ∧
-    HD tr = (s with clock := 0, (t_to_small_t t)) ∧
-    res_rel_t r (LAST tr)`,
+Triviality big_small_lem:
+  !s t r.
+    sem_t s t = r
+    ⇒
+    ?tr.
+      tr ≠ [] ∧
+      s.clock - (SND r).clock ≤ LENGTH tr ∧
+      check_trace (\st. some st'. ?l. step_t st l st') tr ∧
+      HD tr = (s with clock := 0, (t_to_small_t t)) ∧
+      res_rel_t r (LAST tr)
+Proof
  ho_match_mp_tac sem_t_ind >>
  rw [sem_t_def_with_stop, t_to_small_t_def]
  >-
-   (qabbrev_tac`r = sem_e s e`>>fs[markerTheory.Abbrev_def]>>
+   (qabbrev_tac‘r = sem_e s e’>>fs[markerTheory.Abbrev_def]>>
    pop_assum (assume_tac o SYM)>>
    imp_res_tac sem_e_big_small_lem>>
-   Cases_on`r`>>
-   qexists_tac`MAP (λst,e. (st,Exp e)) tr`>>
+   Cases_on‘r’>>
+   qexists_tac‘MAP (λst,e. (st,Exp e)) tr’>>
    imp_res_tac sem_e_clock>>fs[HD_MAP,LAST_MAP]>>
    CONJ_TAC>-
      fs[check_trace_exp]
@@ -992,50 +1015,50 @@ val big_small_lem = Q.prove (
    imp_res_tac step_e_zero_clock>>
    fs[Once step_t_cases])
  >-
-   (qpat_abbrev_tac`A = (s with clock:=0,D)`>>
-   qexists_tac`A::tr`>>fs[Abbr`A`,check_trace_def]>>
+   (qpat_abbrev_tac‘A = (s with clock:=0,D)’>>
+   qexists_tac‘A::tr’>>fs[Abbr‘A’,check_trace_def]>>
    CONJ_TAC >-
-     (Cases_on`tr`>>
+     (Cases_on‘tr’>>
      simp[check_trace_def,optionTheory.some_def]>>
      ntac 2 (simp[Once step_t_cases])>>
      fs[])>>
    fs[LAST_DEF])
  >-
-   (qexists_tac`[s with clock:=0,Break]`>>
+   (qexists_tac‘[s with clock:=0,Break]’>>
    fs[res_rel_t_cases,check_trace_def])
  >-
    (EVERY_CASE_TAC>>fs[]
    >-
-     (qpat_abbrev_tac`p = t_to_small_t t'`>>
-     qexists_tac`MAP (λst,t. (st,Seq t p)) tr ++ tr'`>>
+     (qpat_abbrev_tac‘p = t_to_small_t t'’>>
+     qexists_tac‘MAP (λst,t. (st,Seq t p)) tr ++ tr'’>>
      fs[HD_MAP,HD_APPEND,LAST_APPEND]>>rw[] >>
      match_mp_tac check_trace_append2>>
      fs[check_trace_seq,LAST_MAP]>>
-     Cases_on`LAST tr`>>fs[]>>
+     Cases_on‘LAST tr’>>fs[]>>
      match_mp_tac some_to_SOME_step_t>>
-     simp[Once step_t_cases]>>fs[Abbr`p`,res_rel_t_cases]>>
+     simp[Once step_t_cases]>>fs[Abbr‘p’,res_rel_t_cases]>>
      metis_tac[])
    >-
-     (qpat_abbrev_tac `p = t_to_small_t t'`>>
-     qexists_tac`(MAP (λst,t. (st,Seq t p)) tr)++[r with clock:=0,Break]`>>
+     (qpat_abbrev_tac ‘p = t_to_small_t t'’>>
+     qexists_tac‘(MAP (λst,t. (st,Seq t p)) tr)++[r with clock:=0,Break]’>>
      fs[HD_APPEND,HD_MAP, res_rel_t_cases]>>rw[] >>
      match_mp_tac check_trace_append2>>
      fs[check_trace_seq,LAST_MAP,check_trace_def]>>
      fs[res_rel_t_cases]>>
      match_mp_tac some_to_SOME_step_t>>
-     simp[Once step_t_cases]>>fs[Abbr`p`,res_rel_t_cases])
+     simp[Once step_t_cases]>>fs[Abbr‘p’,res_rel_t_cases])
    >-
-     (qpat_abbrev_tac `p = t_to_small_t t'`>>
-     qexists_tac`(MAP (λst,t. (st,Seq t p)) tr)`>>
+     (qpat_abbrev_tac ‘p = t_to_small_t t'’>>
+     qexists_tac‘(MAP (λst,t. (st,Seq t p)) tr)’>>
      fs[HD_APPEND,HD_MAP,check_trace_def,check_trace_seq]>>rw[]>>
      fs[Once res_rel_t_cases,LAST_MAP]>>
-     rename1 `step_t _ _ (s',_)` >>
-     `step_t (r,Seq t'' p) l (s',Seq t''' p)` by
+     rename1 ‘step_t _ _ (s',_)’ >>
+     ‘step_t (r,Seq t'' p) l (s',Seq t''' p)’ by
        simp[Once step_t_cases]>>
      metis_tac[])
    >-
-     (qpat_abbrev_tac `p = t_to_small_t t'`>>
-     qexists_tac`(MAP (λst,t. (st,Seq t p)) tr)`>>
+     (qpat_abbrev_tac ‘p = t_to_small_t t'’>>
+     qexists_tac‘(MAP (λst,t. (st,Seq t p)) tr)’>>
      fs[HD_APPEND,HD_MAP,check_trace_def,check_trace_seq]>>rw[]>>
      fs[Once res_rel_t_cases,LAST_MAP,is_val_t_def]>>
      metis_tac[no_step_t_seq]))
@@ -1043,11 +1066,11 @@ val big_small_lem = Q.prove (
    (EVERY_CASE_TAC>>fs[sem_e_not_break,sem_e_not_timeout]>>
    imp_res_tac sem_e_big_small_lem>>
    imp_res_tac sem_e_clock>>
-   qpat_abbrev_tac`p1 = t_to_small_t t1`>>
-   qpat_abbrev_tac`p2 = t_to_small_t t2`>>
+   qpat_abbrev_tac‘p1 = t_to_small_t t1’>>
+   qpat_abbrev_tac‘p2 = t_to_small_t t2’>>
    TRY
      (
-     qexists_tac`(MAP (λst,e. (st,(If e p1 p2))) tr') ++ tr`>>
+     qexists_tac‘(MAP (λst,e. (st,(If e p1 p2))) tr') ++ tr’>>
      fs[HD_MAP,HD_APPEND,LAST_MAP,LAST_APPEND]>>rw[] >>
      match_mp_tac check_trace_append2>>fs[res_rel_e_cases]>>CONJ_TAC
      >- metis_tac[check_trace_if1]
@@ -1056,31 +1079,31 @@ val big_small_lem = Q.prove (
          metis_tac[]
      )
    >>
-     qexists_tac`(MAP (λst,e. (st,(If e p1 p2))) tr)`>>rw[]>>
+     qexists_tac‘(MAP (λst,e. (st,(If e p1 p2))) tr)’>>rw[]>>
      fs[HD_MAP,res_rel_t_cases,LAST_MAP,res_rel_e_cases,is_val_t_def,check_trace_if1,no_step_t_if1]>>
      metis_tac[check_trace_if1,no_step_t_if1,step_e_zero_clock])
   >- ( (*For*)
-    reverse (Cases_on`sem_e s e1`>>Cases_on`q`)>>
+    reverse (Cases_on‘sem_e s e1’>>Cases_on‘q’)>>
     fs[sem_e_not_break,sem_e_not_timeout]>>
-    qpat_abbrev_tac`e1s = e_to_small_e e1`>>
-    qpat_abbrev_tac`e2s = e_to_small_e e2`>>
+    qpat_abbrev_tac‘e1s = e_to_small_e e1’>>
+    qpat_abbrev_tac‘e2s = e_to_small_e e2’>>
     (*trace for e1*)
     imp_res_tac sem_e_big_small_lem>>
     imp_res_tac sem_e_clock>>
-    qpat_abbrev_tac`p = t_to_small_t t`>>
-    qabbrev_tac `
+    qpat_abbrev_tac‘p = t_to_small_t t’>>
+    qabbrev_tac ‘
       e1tr = (MAP (λst,e. (st,Handle
-        (If e (Seq p (Seq (Exp e2s) (For e1s e2s p))) (Exp (Num 0))))) tr)`>>
-    `check_trace (λst. some st'. ∃l. step_t st l st') e1tr` by metis_tac[check_trace_for1]>>
-    qabbrev_tac`ls = [s with clock:=0,For e1s e2s p]`>>
-    `check_trace (λst. some st'. ∃l. step_t st l st') (ls++e1tr)` by (
+        (If e (Seq p (Seq (Exp e2s) (For e1s e2s p))) (Exp (Num 0))))) tr)’>>
+    ‘check_trace (λst. some st'. ∃l. step_t st l st') e1tr’ by metis_tac[check_trace_for1]>>
+    qabbrev_tac‘ls = [s with clock:=0,For e1s e2s p]’>>
+    ‘check_trace (λst. some st'. ∃l. step_t st l st') (ls++e1tr)’ by (
       match_mp_tac check_trace_append2>>unabbrev_all_tac>>
       fs[check_trace_def,HD_MAP]>>
       match_mp_tac some_to_SOME_step_t>>
       simp[Once step_t_cases]
       )
     >- (
-      qexists_tac` ls ++ e1tr`>>
+      qexists_tac‘ ls ++ e1tr’>>
       unabbrev_all_tac>>fs[res_rel_t_cases,LAST_DEF,LAST_MAP,HD_APPEND]>>
       fs[LAST_APPEND,LAST_MAP,res_rel_e_cases,is_val_t_def]>>
       match_mp_tac no_step_t_handle>>fs[is_val_t_def]>>
@@ -1090,8 +1113,8 @@ val big_small_lem = Q.prove (
     IF_CASES_TAC>>fs[]
     >- ( (*run out of time*)
       fs[res_rel_t_cases,res_rel_e_cases]>>
-      qexists_tac` (ls ++ e1tr) ++
-        [(r with clock:=0,Handle(Exp (Num 0)));(r with clock:=0,Exp (Num 0))]`>>
+      qexists_tac‘ (ls ++ e1tr) ++
+        [(r with clock:=0,Handle(Exp (Num 0)));(r with clock:=0,Exp (Num 0))]’>>
       fs[LAST_APPEND,LAST_MAP]>>fs[]>>rw[]
       >- (
         match_mp_tac check_trace_append2>>rw[]
@@ -1108,11 +1131,11 @@ val big_small_lem = Q.prove (
         )
        >- (unabbrev_all_tac>>fs[HD_APPEND])
       ) >>
-    reverse (Cases_on`sem_t r t`>>Cases_on`q`)>>fs[]>>
-    qabbrev_tac`ttr = (MAP (λst,t. (st,Handle (Seq t (Seq (Exp e2s) (For e1s e2s p))) ))) tr'`>>
-    `check_trace (λst. some st'. ∃l. step_t st l st') ttr` by
+    reverse (Cases_on‘sem_t r t’>>Cases_on‘q’)>>fs[]>>
+    qabbrev_tac‘ttr = (MAP (λst,t. (st,Handle (Seq t (Seq (Exp e2s) (For e1s e2s p))) ))) tr'’>>
+    ‘check_trace (λst. some st'. ∃l. step_t st l st') ttr’ by
       metis_tac[check_trace_for2]>>
-    `check_trace (λst. some st'. ∃l. step_t st l st') (ls++e1tr++ttr)` by (
+    ‘check_trace (λst. some st'. ∃l. step_t st l st') (ls++e1tr++ttr)’ by (
       match_mp_tac check_trace_append2>>
       fs[]>> unabbrev_all_tac>>
       fs[LAST_MAP,res_rel_e_cases,HD_MAP,LAST_DEF]>>
@@ -1120,22 +1143,22 @@ val big_small_lem = Q.prove (
       ntac 2 (simp[Once step_t_cases])
       )
     >- (
-      qexists_tac`ls++e1tr++ttr`>>unabbrev_all_tac>>
+      qexists_tac‘ls++e1tr++ttr’>>unabbrev_all_tac>>
       fs[LAST_APPEND,LAST_MAP,res_rel_t_cases]>>CONJ_TAC >>
       fs[is_val_t_def]>>match_mp_tac no_step_t_handle>>
       fs[is_val_t_def]>>match_mp_tac no_step_t_seq>>
       metis_tac[]
       )
     >- (
-      qexists_tac`ls++e1tr++ttr`>>unabbrev_all_tac>>
+      qexists_tac‘ls++e1tr++ttr’>>unabbrev_all_tac>>
       fs[LAST_APPEND,LAST_MAP,res_rel_t_cases] >>
       ntac 2 (simp[Once step_t_cases,is_val_t_def])>>
       metis_tac[]
       )
     >- (
-      qexists_tac`
+      qexists_tac‘
         ls++e1tr++ttr++
-          [(r' with clock:= 0,Handle Break);(r' with clock:=0,Exp (Num 0))]`>>
+          [(r' with clock:= 0,Handle Break);(r' with clock:=0,Exp (Num 0))]’>>
       fs[LAST_APPEND,LAST_MAP,res_rel_t_cases]>>rw[]
       >- (unabbrev_all_tac>>fs[]>>DECIDE_TAC)
       >- (
@@ -1147,22 +1170,22 @@ val big_small_lem = Q.prove (
       >- (unabbrev_all_tac>>fs[]>>DECIDE_TAC)
       ) >>
     (*continue executing*)
-    reverse (Cases_on`sem_e r' e2`>>Cases_on`q`)>>
+    reverse (Cases_on‘sem_e r' e2’>>Cases_on‘q’)>>
     fs[sem_e_not_break,sem_e_not_timeout]>>
     imp_res_tac sem_e_big_small_lem>>
     imp_res_tac sem_e_clock>>
-    qabbrev_tac`
-      e2tr = (MAP (λst,e. (st,Handle (Seq (Exp e) (For e1s e2s p)) ))) tr''`>>
-    `check_trace (λst. some st'. ∃l. step_t st l st') e2tr` by
+    qabbrev_tac‘
+      e2tr = (MAP (λst,e. (st,Handle (Seq (Exp e) (For e1s e2s p)) ))) tr''’>>
+    ‘check_trace (λst. some st'. ∃l. step_t st l st') e2tr’ by
       metis_tac[check_trace_for3]>>
-    `check_trace (λst. some st'. ∃l. step_t st l st')(ls++e1tr++ttr++e2tr)` by (
+    ‘check_trace (λst. some st'. ∃l. step_t st l st')(ls++e1tr++ttr++e2tr)’ by (
       match_mp_tac check_trace_append2>>fs[]>>
       match_mp_tac some_to_SOME_step_t>>
       unabbrev_all_tac>>fs[LAST_APPEND,LAST_MAP,HD_MAP,res_rel_t_cases]>>
       ntac 2 (simp[Once step_t_cases,res_rel_e_cases])
       )
     >- ( (* e2 fails *)
-      qexists_tac`ls++e1tr++ttr++e2tr`>>fs[res_rel_e_cases]>>
+      qexists_tac‘ls++e1tr++ttr++e2tr’>>fs[res_rel_e_cases]>>
       unabbrev_all_tac>>
       fs[LAST_APPEND,LAST_MAP,res_rel_t_cases,is_val_t_def]>>rw[] >>
       imp_res_tac step_e_zero_clock>>
@@ -1173,10 +1196,10 @@ val big_small_lem = Q.prove (
     >- (
       (*clock ended*)
       fs[res_rel_t_cases]>>
-      qexists_tac`ls++e1tr++ttr++e2tr`>>fs[]>>reverse (rw[])
+      qexists_tac‘ls++e1tr++ttr++e2tr’>>fs[]>>reverse (rw[])
       >- (
         unabbrev_all_tac>>fs[LAST_APPEND,LAST_MAP,res_rel_e_cases]>>
-        `r'' with clock:=0 = r''` by fs[state_component_equality]>>
+        ‘r'' with clock:=0 = r''’ by fs[state_component_equality]>>
         ntac 2 (simp[Once step_t_cases,is_val_t_def])>>
         metis_tac[]
         ) >>
@@ -1187,11 +1210,11 @@ val big_small_lem = Q.prove (
     simp[Once sem_t_def_with_stop]>>
     fs[dec_clock_def]>>
     (*Need a handle wrapper around rest of trace*)
-    qabbrev_tac`ftr = MAP (λst,t. (st, Handle t))tr''''` >>
-    `check_trace (λst. some st'. ∃l. step_t st l st') ftr` by
+    qabbrev_tac‘ftr = MAP (λst,t. (st, Handle t))tr''''’ >>
+    ‘check_trace (λst. some st'. ∃l. step_t st l st') ftr’ by
       metis_tac[check_trace_handle]>>
-    `check_trace (λst. some st'. ∃l. step_t st l st')
-      (ls++e1tr++ttr++e2tr++ftr)` by (
+    ‘check_trace (λst. some st'. ∃l. step_t st l st')
+      (ls++e1tr++ttr++e2tr++ftr)’ by (
         match_mp_tac check_trace_append2>>fs[]>>
         match_mp_tac some_to_SOME_step_t>>
         unabbrev_all_tac>>fs[LAST_APPEND,LAST_MAP,HD_MAP]>>
@@ -1201,8 +1224,8 @@ val big_small_lem = Q.prove (
     fs[res_rel_t_cases]
     (*Case split on the rest of loop*)
     >- (
-      qexists_tac`
-        ls ++ e1tr ++ ttr ++ e2tr ++ ftr ++[s' with clock:=0,Exp (Num i''')]`>>
+      qexists_tac‘
+        ls ++ e1tr ++ ttr ++ e2tr ++ ftr ++[s' with clock:=0,Exp (Num i''')]’>>
       fs[]>>rw[]
       >- (unabbrev_all_tac>>fs[]>>DECIDE_TAC)
       >- (
@@ -1215,7 +1238,7 @@ val big_small_lem = Q.prove (
       >- (simp[Once sem_t_def_with_stop,LAST_APPEND,dec_clock_def])
       )
     >- (
-      qexists_tac`ls ++ e1tr++ttr++e2tr++ftr`>>fs[]>> reverse (rw[])
+      qexists_tac‘ls ++ e1tr++ttr++e2tr++ftr’>>fs[]>> reverse (rw[])
       >- (
         ntac 4 (simp[Once sem_t_def_with_stop,LAST_APPEND,dec_clock_def])>>
         unabbrev_all_tac>>fs[LAST_APPEND,LAST_MAP,is_val_t_def]>>
@@ -1225,20 +1248,20 @@ val big_small_lem = Q.prove (
       unabbrev_all_tac>>fs[]>>DECIDE_TAC
       )
     >- ( (*break never occurs*)
-      qpat_x_assum `A = (RBreak,s')` mp_tac>>
-      fct>>Cases_on`q`>>
+      qpat_x_assum ‘A = (RBreak,s')’ mp_tac>>
+      fct>>Cases_on‘q’>>
       fs[sem_e_not_timeout,sem_e_not_break]>>
       IF_CASES_TAC>>fs[]>>
-      fct>>Cases_on`q`>>
+      fct>>Cases_on‘q’>>
       fs[]>>
-      fct>>Cases_on`q`>>
+      fct>>Cases_on‘q’>>
       fs[sem_e_not_timeout,sem_e_not_break]>>
       IF_CASES_TAC>>fs[]>>
       simp[STOP_def]>>
       metis_tac[sem_t_for_no_break]
       )
     >- (
-      qexists_tac`ls ++ e1tr ++ ttr ++ e2tr ++ ftr`>>fs[]>> reverse (rw[]) >>
+      qexists_tac‘ls ++ e1tr ++ ttr ++ e2tr ++ ftr’>>fs[]>> reverse (rw[]) >>
       unabbrev_all_tac
       >- (
         ntac 3 (
@@ -1248,13 +1271,14 @@ val big_small_lem = Q.prove (
       fs[] >> DECIDE_TAC
       )
     )
-  )
+QED
 
-val big_timeout_0 = Q.prove (
-`!st p r.
-  sem_t st p = (Rtimeout,r)
-  ⇒
-  r.clock = 0`,
+Triviality big_timeout_0:
+  !st p r.
+    sem_t st p = (Rtimeout,r)
+    ⇒
+    r.clock = 0
+Proof
  ho_match_mp_tac sem_t_ind >>
  conj_tac >- (
    rw [sem_t_def_with_stop, sem_e_not_timeout]) >>
@@ -1276,296 +1300,327 @@ val big_timeout_0 = Q.prove (
    ect >>
    fs [sem_e_not_timeout, STOP_def] >>
    rw [] >>
-   fs []));
+   fs [])
+QED
 
 (* check traces are unique up to prefixing *)
-val check_trace_determ = Q.prove(
-`∀tr h f.
- check_trace f (h::tr) ⇒
- ∀tr'.
- LENGTH tr' ≤ LENGTH tr ∧
- check_trace f (h::tr') ⇒
- isPREFIX tr' tr`,
+Triviality check_trace_determ:
+  ∀tr h f.
+    check_trace f (h::tr) ⇒
+    ∀tr'.
+      LENGTH tr' ≤ LENGTH tr ∧
+      check_trace f (h::tr') ⇒
+      isPREFIX tr' tr
+Proof
  Induct>>rw[]>>fs[check_clock_def,isPREFIX,LENGTH_NIL]>>
- Cases_on`tr'`>>fs[check_trace_def]>>
- metis_tac[])
+ Cases_on‘tr'’>>fs[check_trace_def]>>
+ metis_tac[]
+QED
 
-val check_trace_prefixes = Q.prove(
-`∀tr f.
- tr ≠ [] ∧
- check_trace f tr ⇒
- ∀tr'.
- tr' ≠ [] ∧ HD tr' = HD tr ∧
- check_trace f tr' ⇒
- isPREFIX tr tr' ∨ isPREFIX tr' tr`,
- rw[]>>
- Cases_on`tr`>>Cases_on`tr'`>>fs[]>>
- Cases_on`LENGTH t' ≤ LENGTH t`>>
- TRY(`LENGTH t ≤ LENGTH t'` by DECIDE_TAC)>>
- metis_tac[check_trace_determ])
+Triviality check_trace_prefixes:
+  ∀tr f.
+    tr ≠ [] ∧
+    check_trace f tr ⇒
+    ∀tr'.
+      tr' ≠ [] ∧ HD tr' = HD tr ∧
+      check_trace f tr' ⇒
+      isPREFIX tr tr' ∨ isPREFIX tr' tr
+Proof
+  rw[]>>
+  Cases_on‘tr’>>Cases_on‘tr'’>>fs[]>>
+  Cases_on‘LENGTH t' ≤ LENGTH t’>>
+  TRY(‘LENGTH t ≤ LENGTH t'’ by DECIDE_TAC)>>
+  metis_tac[check_trace_determ]
+QED
 
-val check_trace_TL = Q.prove(
-`∀tr tr'.
- (tr ≠ [] ∧
- check_trace (λst. some st'. ?l. step_t st l st') tr ∧
- (∀l t'. ¬step_t (LAST tr) l t') ∧
- check_trace (λst. some st'. ?l. step_t st l st') tr' ∧
- isPREFIX tr tr') ⇒
- tr = tr'`,
- Induct>>fs[check_trace_def,LAST_DEF]>>rw[]>>Cases_on`tr'`>>fs[]
- >-
-   (Cases_on`t`>>fs[check_trace_def,some_def]>>
-   metis_tac[])
- >>
-   Cases_on`tr`>>Cases_on`t`>>fs[check_trace_def]>>
-   res_tac>>fs[])
+Triviality check_trace_TL:
+  ∀tr tr'.
+    tr ≠ [] ∧
+    check_trace (λst. some st'. ?l. step_t st l st') tr ∧
+    (∀l t'. ¬step_t (LAST tr) l t') ∧
+    check_trace (λst. some st'. ?l. step_t st l st') tr' ∧
+    isPREFIX tr tr' ⇒
+    tr = tr'
+Proof
+  Induct>>fs[check_trace_def,LAST_DEF]>>rw[]>>Cases_on‘tr'’>>fs[]
+  >-
+   (Cases_on‘t’>>fs[check_trace_def,some_def]>>
+    metis_tac[])
+  >>
+  Cases_on‘tr’>>Cases_on‘t’>>fs[check_trace_def]>>
+  res_tac>>fs[]
+QED
 
-val prefix_append = Q.prove(
-`∀ls ls'.
-  ls ≼ ls' ⇒
-  ∃ls''. ls++ls'' = ls'`,
-  metis_tac[rich_listTheory.IS_PREFIX_APPEND])
+Triviality prefix_append:
+  ∀ls ls'. ls ≼ ls' ⇒ ∃ls''. ls++ls'' = ls'
+Proof
+  metis_tac[rich_listTheory.IS_PREFIX_APPEND]
+QED
 
-val res_rel_t_io_trace = Q.prove(
- `res_rel_t (q,r) s ⇒
-  r.io_trace = (FST s).io_trace`,
-  simp[res_rel_t_cases]>>rw[]>>fs[])
+Triviality res_rel_t_io_trace:
+  res_rel_t (q,r) s ⇒ r.io_trace = (FST s).io_trace
+Proof
+  simp[res_rel_t_cases]>>rw[]>>fs[]
+QED
 
 (*slow*)
-val res_rel_t_clock = Q.prove(
- `res_rel_t (q,r) s ∧
+Triviality res_rel_t_clock:
+ res_rel_t (q,r) s ∧
   step_t s l t ⇒
-  q = Rtimeout ∧ (FST s).clock = 0`,
-  simp[res_rel_t_cases]>>rw[]
-  >>
-    fs[Once step_t_cases,Once step_e_cases]
-  >>
-   metis_tac[PAIR,FST])
+  q = Rtimeout ∧ (FST s).clock = 0
+Proof
+  simp[res_rel_t_cases]>>rw[] >>
+  fs[Once step_t_cases,Once step_e_cases] >>
+  metis_tac[PAIR,FST]
+QED
 
-val step_e_io_mono = Q.prove(
-`∀s l s'.
-  step_e s l s' ⇒
-  (FST s).io_trace ≼ (FST s').io_trace`,
-  ho_match_mp_tac step_e_strongind>>fs[])
+Triviality step_e_io_mono:
+  ∀s l s'.
+    step_e s l s' ⇒
+    (FST s).io_trace ≼ (FST s').io_trace
+Proof
+  Induct_on ‘step_e’ >> simp[]
+QED
 
-val step_t_io_mono = Q.prove(
-`∀s l s'.
-  step_t s l s' ⇒
-  (FST s).io_trace ≼ (FST s').io_trace`,
-  ho_match_mp_tac step_t_strongind>>
-  fs[]>>metis_tac[step_e_io_mono,FORALL_PROD,FST])
+Triviality step_t_io_mono:
+  ∀s l s'.
+    step_t s l s' ⇒
+    (FST s).io_trace ≼ (FST s').io_trace
+Proof
+  Induct_on ‘step_t’ >> simp[] >>
+  metis_tac[step_e_io_mono,FORALL_PROD,FST]
+QED
 
-val RTC_step_t_io_mono = Q.prove(
-  `∀x y. (λs1 s2. (some st'. ∃l. step_t s1 l st') = SOME s2)^* x y ⇒
-      (FST x).io_trace ≼ (FST y).io_trace`,
-  ho_match_mp_tac RTC_INDUCT >> rw[] >>
+Triviality RTC_step_t_io_mono:
+  ∀x y. (λs1 s2. (some st'. ∃l. step_t s1 l st') = SOME s2)^* x y ⇒
+        (FST x).io_trace ≼ (FST y).io_trace
+Proof
+  Induct_on ‘RTC’ >> rw[] >>
   last_x_assum mp_tac >>
   DEEP_INTRO_TAC some_intro >> rw[] >>
-  metis_tac[step_t_io_mono,IS_PREFIX_TRANS])
+  metis_tac[step_t_io_mono,IS_PREFIX_TRANS]
+QED
 
-val check_trace_io_trace = Q.prove(
- `∀tr ls.
-  tr ≠ [] ∧ check_trace (λst. some st'. ∃l. step_t st l st') (tr ++ ls) ⇒
-  (FST(LAST tr)).io_trace ≼
-  (FST(LAST (tr++ls))).io_trace`,
+Triviality check_trace_io_trace:
+  ∀tr ls.
+    tr ≠ [] ∧ check_trace (λst. some st'. ∃l. step_t st l st') (tr ++ ls) ⇒
+    (FST(LAST tr)).io_trace ≼ (FST(LAST (tr++ls))).io_trace
+Proof
   rw[] >>
   match_mp_tac RTC_step_t_io_mono >>
   simp[check_trace_thm] >>
-  qexists_tac`LAST tr::ls` >>
+  qexists_tac‘LAST tr::ls’ >>
   simp[] >>
-  conj_tac >- ( Cases_on`ls`>>simp[] ) >>
-  `LAST tr::ls = DROP (LENGTH tr - 1) (tr++ls)` suffices_by (
+  conj_tac >- ( Cases_on‘ls’>>simp[] ) >>
+  ‘LAST tr::ls = DROP (LENGTH tr - 1) (tr++ls)’ suffices_by (
     disch_then SUBST1_TAC >>
     match_mp_tac check_trace_drop >> simp[] ) >>
   simp[DROP_APPEND1] >>
-  Q.ISPECL_THEN[`1n`,`tr`]mp_tac (GSYM LASTN_DROP) >>
-  `1 ≤ LENGTH tr` by (
-    Cases_on`tr`>>fs[] >> simp[] ) >>
+  Q.ISPECL_THEN[‘1n’,‘tr’]mp_tac (GSYM LASTN_DROP) >>
+  ‘1 ≤ LENGTH tr’ by (
+    Cases_on‘tr’>>fs[] >> simp[] ) >>
   simp[] >>
-  Q.ISPEC_THEN`tr`FULL_STRUCT_CASES_TAC SNOC_CASES >- fs[] >>
-  REWRITE_TAC[arithmeticTheory.ONE,LASTN,LAST,SNOC])
+  Q.ISPEC_THEN‘tr’FULL_STRUCT_CASES_TAC SNOC_CASES >- fs[] >>
+  REWRITE_TAC[arithmeticTheory.ONE,LASTN,LAST,SNOC]
+QED
 
-val sem_e_ignores_clock = Q.prove(
- `∀s e c r s'.
-  sem_e s e = (r,s') ⇒
-  sem_e (s with clock:=c) e = (r,s' with clock:=c)`,
+Triviality sem_e_ignores_clock:
+  ∀s e c r s'.
+    sem_e s e = (r,s') ⇒
+    sem_e (s with clock:=c) e = (r,s' with clock:=c)
+Proof
   ho_match_mp_tac sem_e_ind>>srw_tac[][sem_e_def]>>fs[LET_THM]
   >-
     (ect>>fs[])
-  >- (
-    fs[permute_pair_def,LET_THM,oracle_get_def,unpermute_pair_def]>>
-    Cases_on`switch`>>fs[]>>
-    qpat_x_assum`A=(r,s')` mp_tac>>
-    fct>>Cases_on`q`>>res_tac>>
-    fs[sem_e_not_break,sem_e_not_timeout]>>
-    fct>>Cases_on`q`>>res_tac>>
-    rw[]>>
-    fs[sem_e_not_break,sem_e_not_timeout])
+  >- (fs[permute_pair_def,LET_THM,oracle_get_def,unpermute_pair_def]>>
+      Cases_on‘switch’>>fs[]>>
+      qpat_x_assum‘A=(r,s')’ mp_tac>>
+      fct>>Cases_on‘q’>>res_tac>>
+      fs[sem_e_not_break,sem_e_not_timeout]>>
+      fct>>Cases_on‘q’>>res_tac>>
+      rw[]>>
+      fs[sem_e_not_break,sem_e_not_timeout])
   >>
-    Cases_on`sem_e s e`>>res_tac>>fs[]>>
-    Cases_on`q`>>fs[state_component_equality])
+    Cases_on‘sem_e s e’>>res_tac>>fs[]>>
+    Cases_on‘q’>>fs[state_component_equality]
+QED
 
-val sem_e_io_mono = Q.prove(
-  `∀s e c.
-  (SND (sem_e s e)).io_trace ≼
-  (SND (sem_e (s with clock:= c) e)).io_trace`,
-  rw[]>>Cases_on`sem_e s e`>>imp_res_tac sem_e_ignores_clock>>
-  fs[])
+Triviality sem_e_io_mono:
+  ∀s e c.
+    (SND (sem_e s e)).io_trace ≼ (SND (sem_e (s with clock:= c) e)).io_trace
+Proof
+  rw[]>>Cases_on‘sem_e s e’>>imp_res_tac sem_e_ignores_clock>>
+  fs[]
+QED
 
-val sem_e_clock_inc = Q.prove(
-  `∀s e r.
-  sem_e s e = r ⇒
-  ∀k. sem_e (s with clock:= s.clock+k) e =(FST r,(SND r)with clock:= (SND r).clock+k)`,
-  metis_tac[sem_e_ignores_clock,sem_e_clock,FST,SND,PAIR])
+Triviality sem_e_clock_inc:
+  ∀s e r.
+    sem_e s e = r ⇒
+    ∀k. sem_e (s with clock:= s.clock+k) e =
+        (FST r, (SND r) with clock:= (SND r).clock+k)
+Proof
+  metis_tac[sem_e_ignores_clock,sem_e_clock,FST,SND,PAIR]
+QED
 
-val sem_t_clock_inc = Q.prove(
-  `∀s t r.
-  sem_t s t = r ∧ FST r ≠ Rtimeout ⇒
-  ∀k. sem_t (s with clock:= s.clock+k) t =(FST r,(SND r)with clock:= (SND r).clock+k)`,
+Triviality sem_t_clock_inc:
+  ∀s t r.
+    sem_t s t = r ∧ FST r ≠ Rtimeout ⇒
+    ∀k. sem_t (s with clock:= s.clock+k) t =
+        (FST r, (SND r) with clock:= (SND r).clock+k)
+Proof
   ho_match_mp_tac sem_t_ind>>rw[]>>fs[sem_e_clock]>>
   TRY(fs[sem_t_def_with_stop]>>NO_TAC)
   >-
     (fs[sem_t_def_with_stop]>>
-    Cases_on`sem_e s e`>>
+    Cases_on‘sem_e s e’>>
     imp_res_tac sem_e_ignores_clock>>
     fs[]>>metis_tac[sem_e_clock])
   >-
-    (fs[sem_t_def_with_stop]>>Cases_on`sem_t s t`>>Cases_on`q`>>fs[])
+    (fs[sem_t_def_with_stop]>>Cases_on‘sem_t s t’>>Cases_on‘q’>>fs[])
   >-
-    (fs[sem_t_def_with_stop]>>Cases_on`sem_e s e`>>Cases_on`q`>>fs[sem_e_res]>>
+    (fs[sem_t_def_with_stop]>>Cases_on‘sem_e s e’>>Cases_on‘q’>>fs[sem_e_res]>>
     imp_res_tac sem_e_clock_inc>>
-    pop_assum(qspec_then`k` assume_tac)>>fs[]>>
+    pop_assum(qspec_then‘k’ assume_tac)>>fs[]>>
     IF_CASES_TAC>>fs[])
   >>
     pop_assum mp_tac>>
     simp[sem_t_def_with_stop]>>
-    Cases_on`sem_e s e1`>>Cases_on`q`>>fs[]>>
+    Cases_on‘sem_e s e1’>>Cases_on‘q’>>fs[]>>
     imp_res_tac sem_e_clock_inc>>fs[]>>
-    TRY(pop_assum(qspec_then`k` assume_tac))>>
-    fs[DECIDE ``(A:num)+B = B+A``]>>
+    TRY(pop_assum(qspec_then‘k’ assume_tac))>>
+    fs[DECIDE “(A:num)+B = B+A”]>>
     IF_CASES_TAC>>fs[]>>
-    Cases_on`sem_t r t`>>Cases_on`q`>>fs[]>>
-    Cases_on`sem_e r' e2`>>Cases_on`q`>>fs[]>>
+    Cases_on‘sem_t r t’>>Cases_on‘q’>>fs[]>>
+    Cases_on‘sem_e r' e2’>>Cases_on‘q’>>fs[]>>
     TRY(metis_tac[sem_e_res])>>
     imp_res_tac sem_e_clock_inc>>fs[]>>
-    TRY(pop_assum(qspec_then`k` assume_tac))>>
-    fs[DECIDE ``(A:num)+B = B+A``]>>
+    TRY(pop_assum(qspec_then‘k’ assume_tac))>>
+    fs[DECIDE “(A:num)+B = B+A”]>>
     IF_CASES_TAC>>fs[]>>rw[]>>
     fs[dec_clock_def,STOP_def]>>
-    `1 ≤ r''.clock` by DECIDE_TAC>>
-    metis_tac[arithmeticTheory.LESS_EQ_ADD_SUB])
+    ‘1 ≤ r''.clock’ by DECIDE_TAC>>
+    metis_tac[arithmeticTheory.LESS_EQ_ADD_SUB]
+QED
 
-val check_trace_io_trace_simp = Q.prove(
-  `tr ≠ [] ∧
+Triviality check_trace_io_trace_simp:
+  tr ≠ [] ∧
   check_trace (λst.some st'. ∃l. step_t st l st') tr ⇒
-  (FST(HD tr)).io_trace ≼ (FST (LAST tr)).io_trace`,
-  Cases_on`tr`>>rw[]>>
-  `FST h = FST(LAST [h])` by fs[]>>
+  (FST(HD tr)).io_trace ≼ (FST (LAST tr)).io_trace
+Proof
+  Cases_on‘tr’>>rw[]>>
+  ‘FST h = FST(LAST [h])’ by fs[]>>
   pop_assum SUBST1_TAC>>
-  `h::t = [h]++t` by fs[]>>
+  ‘h::t = [h]++t’ by fs[]>>
   pop_assum SUBST1_TAC>>
   ho_match_mp_tac check_trace_io_trace>>
-  rw[])
+  rw[]
+QED
 
-val sem_t_sing_io_mono = Q.prove(
-  `∀s t res s'.
-  sem_t s t = (res,s') ⇒
-  s.io_trace ≼ s'.io_trace`,
+Triviality sem_t_sing_io_mono:
+  ∀s t res s'. sem_t s t = (res,s') ⇒ s.io_trace ≼ s'.io_trace
+Proof
   rw[]>>imp_res_tac big_small_lem>>
   imp_res_tac check_trace_io_trace_simp>>
   fs[res_rel_t_cases]>>
-  rfs[])
+  rfs[]
+QED
 
-val sem_e_sing_io_mono = Q.prove(
-`∀s e res s'.
-  sem_e s e = (res,s') ⇒
-  s.io_trace ≼ s'.io_trace`,
+Triviality sem_e_sing_io_mono:
+  ∀s e res s'. sem_e s e = (res,s') ⇒ s.io_trace ≼ s'.io_trace
+Proof
   CCONTR_TAC>>fs[]>>
-  `sem_t s (Exp e) = (res,s')` by
+  ‘sem_t s (Exp e) = (res,s')’ by
     fs[sem_t_def_with_stop]>>
-  metis_tac[sem_t_sing_io_mono])
+  metis_tac[sem_t_sing_io_mono]
+QED
 
 (* Monotonicity of io_trace w.r.t. to clock *)
-val sem_t_io_mono_lem = Q.prove(
- `∀s t k.
-  (SND (sem_t s t)).io_trace ≼
-  (SND (sem_t (s with clock:=s.clock+k) t)).io_trace`,
+Triviality sem_t_io_mono_lem:
+  ∀s t k.
+    (SND (sem_t s t)).io_trace ≼
+    (SND (sem_t (s with clock:=s.clock+k) t)).io_trace
+Proof
   ho_match_mp_tac sem_t_ind>>rw[]>>
   TRY(fs[sem_t_def_with_stop,sem_e_io_mono]>>NO_TAC)
   >-
     (fs[sem_t_def_with_stop]>>
-    fct>>Cases_on`q`>>fs[]>>
+    fct>>Cases_on‘q’>>fs[]>>
     imp_res_tac sem_t_clock_inc>>fs[]>>
-    fct>>Cases_on`q`>>fs[]>>
-    first_x_assum(qspec_then`k` assume_tac)>>rfs[]>>
-    Cases_on`sem_t r' t'`>>
+    fct>>Cases_on‘q’>>fs[]>>
+    first_x_assum(qspec_then‘k’ assume_tac)>>rfs[]>>
+    Cases_on‘sem_t r' t'’>>
     imp_res_tac sem_t_sing_io_mono>>
     fs[]>>
     metis_tac[IS_PREFIX_TRANS])
   >-
     (fs[sem_t_def_with_stop]>>
-    fct>>Cases_on`q`>>fs[]>>TRY(metis_tac[sem_e_res])>>
+    fct>>Cases_on‘q’>>fs[]>>TRY(metis_tac[sem_e_res])>>
     imp_res_tac sem_e_clock_inc>>fs[]>>
     IF_CASES_TAC>>fs[])
   >>
     simp[Once sem_t_def_with_stop]>>
     simp[Once sem_t_def_with_stop]>>
-    fct>>Cases_on`q`>>fs[]>>TRY(metis_tac[sem_e_res])>>
+    fct>>Cases_on‘q’>>fs[]>>TRY(metis_tac[sem_e_res])>>
     imp_res_tac sem_e_clock_inc>>
-    pop_assum(qspec_then`k` assume_tac)>>
-    fs[DECIDE ``(A:num)+B = B+A``]>>
+    pop_assum(qspec_then‘k’ assume_tac)>>
+    fs[DECIDE “(A:num)+B = B+A”]>>
     IF_CASES_TAC>>fs[]>>
-    fct>>Cases_on`q`>>fs[]>>
+    fct>>Cases_on‘q’>>fs[]>>
     TRY(imp_res_tac sem_t_clock_inc>>fs[]>>
-    pop_assum(qspec_then`k` assume_tac))>>rfs[]>>
-    fs[DECIDE ``(A:num)+B = B+A``]
+    pop_assum(qspec_then‘k’ assume_tac))>>rfs[]>>
+    fs[DECIDE “(A:num)+B = B+A”]
     >-
-      (fct>>Cases_on`q`>>fs[]>>TRY(metis_tac[sem_e_res])>>
+      (fct>>Cases_on‘q’>>fs[]>>TRY(metis_tac[sem_e_res])>>
       imp_res_tac sem_e_clock_inc>>
-      pop_assum(qspec_then`k` assume_tac)>>
-      fs[DECIDE ``(A:num)+B = B+A``]>>
+      pop_assum(qspec_then‘k’ assume_tac)>>
+      fs[DECIDE “(A:num)+B = B+A”]>>
       IF_CASES_TAC>>fs[]
       >-
         (fs[dec_clock_def,STOP_def]>>
-        `1 ≤ r''.clock` by DECIDE_TAC>>
+        ‘1 ≤ r''.clock’ by DECIDE_TAC>>
         metis_tac[arithmeticTheory.LESS_EQ_ADD_SUB])
       >>
       IF_CASES_TAC>>fs[]>>
-      qpat_abbrev_tac`A = sem_t B C`>>
-      Cases_on`A`>>fs[markerTheory.Abbrev_def]>>
+      qpat_abbrev_tac‘A = sem_t B C’>>
+      Cases_on‘A’>>fs[markerTheory.Abbrev_def]>>
       pop_assum (assume_tac o SYM)>>imp_res_tac sem_t_sing_io_mono>>
       fs[dec_clock_def])
     >>
-      first_x_assum(qspec_then`k` assume_tac)>>
-      fct>>Cases_on`q`>>fs[]>>
-      fct>>Cases_on`q`>>fs[]>>TRY(metis_tac[sem_e_res])>>
+      first_x_assum(qspec_then‘k’ assume_tac)>>
+      fct>>Cases_on‘q’>>fs[]>>
+      fct>>Cases_on‘q’>>fs[]>>TRY(metis_tac[sem_e_res])>>
       imp_res_tac sem_e_sing_io_mono
       >-
         (IF_CASES_TAC>>fs[dec_clock_def]>>
-        TRY(qpat_abbrev_tac`A = sem_t B C`>>
-        Cases_on`A`>>fs[markerTheory.Abbrev_def]>>
+        TRY(qpat_abbrev_tac‘A = sem_t B C’>>
+        Cases_on‘A’>>fs[markerTheory.Abbrev_def]>>
         pop_assum (assume_tac o SYM)>>imp_res_tac sem_t_sing_io_mono)>>
         fs[]>>metis_tac[IS_PREFIX_TRANS])
       >>
-      metis_tac[IS_PREFIX_TRANS])
+      metis_tac[IS_PREFIX_TRANS]
+QED
 
-val sem_t_io_mono = Q.prove (
-`k1 ≤ k2 ⇒
- (SND (sem_t (init_st 0 nd input with clock := k1) p)).io_trace ≼
- (SND (sem_t (init_st 0 nd input with clock := k2) p)).io_trace`,
- qpat_abbrev_tac `st = init_st A B C`>>
+Triviality sem_t_io_mono:
+  k1 ≤ k2 ⇒
+  (SND (sem_t (init_st 0 nd input with clock := k1) p)).io_trace ≼
+  (SND (sem_t (init_st 0 nd input with clock := k2) p)).io_trace
+Proof
+ qpat_abbrev_tac ‘st = init_st A B C’>>
  rw[]>>imp_res_tac arithmeticTheory.LESS_EQUAL_ADD >>
- Q.ISPECL_THEN [`st with clock:=k1`,`p`,`p'`] assume_tac sem_t_io_mono_lem>>
- fs[])
+ Q.SPECL_THEN [‘st with clock:=k1’,‘p’,‘p'’] assume_tac sem_t_io_mono_lem>>
+ fs[]
+QED
 
-val sem_equiv_lem = Q.store_thm ("sem_equiv_lem",
-`∀input prog r. ofbs_sem (for_big_sem input) prog r ⇔ osmall_sem (for_small_sem input) prog r`,
+Theorem sem_equiv_lem:
+  ∀input prog r. ofbs_sem (for_big_sem input) prog r ⇔
+                   osmall_sem (for_small_sem input) prog r
+Proof
  gen_tac >>
  match_mp_tac osmall_fbs_equiv2 >>
  conj_tac >- (
    rw [for_small_sem_def] >>
    match_mp_tac step_t_io_mono>>
-   Q.ISPEC_THEN `λst. ∃l. step_t s1 l st` assume_tac some_SAT>>
+   Q.ISPEC_THEN ‘λst. ∃l. step_t s1 l st’ assume_tac some_SAT>>
    fs[ETA_AX])>>
  conj_tac >- (
    rw [for_big_sem_def] >>
@@ -1578,11 +1633,11 @@ val sem_equiv_lem = Q.store_thm ("sem_equiv_lem",
    ect >>
    fs [] >>
    metis_tac [big_timeout_0]) >>
- qexists_tac `I` >>
+ qexists_tac ‘I’ >>
  conj_tac
  >- (
    rw [unbounded_def] >>
-   qexists_tac `SUC x` >>
+   qexists_tac ‘SUC x’ >>
    simp []) >>
  rpt gen_tac >>
  simp [for_big_sem_def, for_eval_def, eval_with_clock_def] >>
@@ -1590,7 +1645,7 @@ val sem_equiv_lem = Q.store_thm ("sem_equiv_lem",
  ect >>
  imp_res_tac big_small_lem >>
  fs [] >>
- qexists_tac `tr` >>
+ qexists_tac ‘tr’ >>
  fs [for_small_sem_def] >>
  rw [same_result_def] >>
  fs [res_rel_t_cases, is_val_t_def, is_val_e_def, some_no_choice, init_st_def] >>
@@ -1601,69 +1656,91 @@ val sem_equiv_lem = Q.store_thm ("sem_equiv_lem",
  >- rw [Once step_t_cases]
  >- (rw [some_def] >>
      metis_tac [])
- >- metis_tac [PAIR]);
+ >- metis_tac [PAIR]
+QED
 
-val FST_SPLIT = Q.prove(
-`FST x = y ⇒ ∃z. x = (y,z)`,
-Cases_on`x`>>fs[])
+Triviality FST_SPLIT: FST x = y ⇒ ∃z. x = (y,z)
+Proof Cases_on‘x’>>fs[]
+QED
 
-val big_val_no_errors = Q.prove(
-`!st p v s.
-  sem_t st p = (Rval v,s)
-  ⇒
-  (∀c.
-    (FST (sem_t (st with clock:= c) p) ≠ Rbreak)
-  ∧ (FST (sem_t (st with clock:=c) p) ≠ Rfail))`,
+Triviality big_val_no_errors:
+  !st p v s.
+    sem_t st p = (Rval v,s)
+   ⇒
+    ∀c.
+      FST (sem_t (st with clock:= c) p) ≠ Rbreak ∧
+      FST (sem_t (st with clock:=c) p) ≠ Rfail
+Proof
   rw[]>>CCONTR_TAC>>fs[]>>imp_res_tac FST_SPLIT>>
   imp_res_tac big_small_lem>>
-  `HD tr = HD tr'` by fs[]>>
+  ‘HD tr = HD tr'’ by fs[]>>
   fs[res_rel_t_cases]>>
-  `∀l t'. ¬step_t (LAST tr) l t'` by
-    fs[Once step_t_cases,FORALL_PROD]>>
-  `∀l t'. ¬step_t (LAST tr') l t'` by
-    fs[Once step_t_cases,FORALL_PROD,Once step_e_cases]>>
-  `isPREFIX tr tr' ∨ isPREFIX tr' tr` by
+  ‘∀l t'. ¬step_t (LAST tr) l t'’ by
+    (simp[Once step_t_cases,FORALL_PROD]>> rw[] >>
+     qpat_x_assum ‘∀a b c. ¬step_t _ _ _ ’ mp_tac >>
+     simp[Once step_t_cases] >> simp[Once step_t_cases, Once step_e_cases]) >>
+  ‘∀l t'. ¬step_t (LAST tr') l t'’ by
+    simp[Once step_t_cases,FORALL_PROD,Once step_e_cases]>>
+  ‘isPREFIX tr tr' ∨ isPREFIX tr' tr’ by
     metis_tac[check_trace_prefixes]>>
-  `tr = tr'` by metis_tac[check_trace_TL]>>
+  ‘tr = tr'’ by metis_tac[check_trace_TL]>>
   fs[]>>
-  qpat_assum`A=t` (SUBST_ALL_TAC o SYM)>>fs[is_val_t_def,is_val_e_def])
+  qpat_assum‘A=t’ (SUBST_ALL_TAC o SYM)>>fs[is_val_t_def,is_val_e_def]
+QED
 
 (* we can prove an alternative characterisation of the semantics, now that we
    know sem_t's io_trace is a chain *)
 
-val over_all_def = Define`over_all f = GSPEC (λc. f c,T)`;
+Definition over_all_def:
+  over_all f = { f c | c | T }
+End
 
-val init_st_with_clock = Q.prove(
-  `init_st a b c with clock := d = init_st d b c`,
-  EVAL_TAC)
+Triviality init_st_with_clock:
+  init_st a b c with clock := d = init_st d b c
+Proof EVAL_TAC
+QED
 
-val lprefix_chain_sem_t_io_trace_over_all_c = Q.store_thm("lprefix_chain_sem_t_io_trace_over_all_c",
-  `prefix_chain (over_all (λc. (SND (sem_t (init_st c nd input) t)).io_trace))`,
+Theorem lprefix_chain_sem_t_io_trace_over_all_c:
+  prefix_chain (over_all (λc. (SND (sem_t (init_st c nd input) t)).io_trace))
+Proof
   rw[lprefix_lubTheory.prefix_chain_def,over_all_def] >>
-  qspecl_then[`c`,`c'`]strip_assume_tac arithmeticTheory.LESS_EQ_CASES >|[disj1_tac,disj2_tac] >>
-  imp_res_tac sem_t_io_mono >> fs[init_st_with_clock])
+  qspecl_then[‘c’,‘c'’]strip_assume_tac arithmeticTheory.LESS_EQ_CASES >|[disj1_tac,disj2_tac] >>
+  imp_res_tac sem_t_io_mono >> fs[init_st_with_clock]
+QED
 
-val image_intro = Q.prove(
-  `{fromList (FILTER P (Q c)) | c | T} = IMAGE fromList (IMAGE (FILTER P) (over_all Q))`,
-  rw[EXTENSION,over_all_def,PULL_EXISTS])
+Triviality image_intro:
+  {fromList (FILTER P (Q c)) | c | T} =
+  IMAGE fromList (IMAGE (FILTER P) (over_all Q))
+Proof
+  rw[EXTENSION,over_all_def,PULL_EXISTS]
+QED
 
-val IMAGE_over_all = Q.store_thm("IMAGE_over_all",
-  `IMAGE P (over_all f) = over_all (P o f)`,
-  rw[EXTENSION,over_all_def,PULL_EXISTS])
+Theorem IMAGE_over_all:
+  IMAGE P (over_all f) = over_all (P o f)
+Proof
+  rw[EXTENSION,over_all_def,PULL_EXISTS]
+QED
 
 (* Pretty Printing *)
-val BIGSUP_def = Define`BIGSUP f = build_lprefix_lub (over_all f)`
+Definition BIGSUP_def: BIGSUP f = build_lprefix_lub (over_all f)
+End
 
-val _ = Parse.add_rule{term_name="BIGSUP",fixity=Parse.Binder,pp_elements=[TOK"BIGSUP"],
-                       block_style=(NoPhrasing,(PP.CONSISTENT,0)),paren_style=OnlyIfNecessary}
+val _ = Parse.add_rule{
+  term_name="BIGSUP", fixity=Parse.Binder,
+  pp_elements=[TOK"BIGSUP"],
+  block_style=(NoPhrasing,(PP.CONSISTENT,0)),paren_style=OnlyIfNecessary
+  }
 
-val semantics_alt = save_thm("semantics_alt",
+Theorem semantics_alt =
   semantics_def
     |> SIMP_RULE bool_ss [image_intro]
-    |> SIMP_RULE bool_ss [lprefix_chain_sem_t_io_trace_over_all_c,lprefix_lubTheory.prefix_chain_FILTER,lprefix_lubTheory.prefix_chain_lprefix_chain,lprefix_lubTheory.build_prefix_lub_intro]
+    |> SIMP_RULE bool_ss [lprefix_chain_sem_t_io_trace_over_all_c,
+                          lprefix_lubTheory.prefix_chain_FILTER,
+                          lprefix_lubTheory.prefix_chain_lprefix_chain,
+                          lprefix_lubTheory.build_prefix_lub_intro]
     |> SIMP_RULE bool_ss [IMAGE_over_all]
-    |> SIMP_RULE bool_ss [prove(``f o g = λc. f (g c)``,rw[FUN_EQ_THM])]
-    |> SIMP_RULE bool_ss [GSYM BIGSUP_def])
+    |> SIMP_RULE bool_ss [prove(“f o g = λc. f (g c)”,rw[FUN_EQ_THM])]
+    |> SIMP_RULE bool_ss [GSYM BIGSUP_def]
 
 Definition oracle_upd_def:
   oracle_upd s (b,a) = s with <|non_det_o := a; io_trace:=s.io_trace ++[INR b]|>
